ChoiceType/theories/Qualifier.v
@@ -37,7 +37,7 @@ Definition qual_subst_one (x : atom) (v : value) (q : type_qualifier) : type_qua
   | qual vals prop => qual (vmap (value_subst x v) vals) prop
   end.
 
-Definition qual_subst (σ : StoreT) (q : type_qualifier) : type_qualifier :=
+Definition qual_subst (σ : Store) (q : type_qualifier) : type_qualifier :=
   match q with
   | qual vals prop => qual (vmap (value_subst_all σ) vals) prop
   end.
@@ -46,7 +46,7 @@ Definition qual_subst (σ : StoreT) (q : type_qualifier) : type_qualifier :=
 #[global] Instance close_qual_inst     : Close type_qualifier := qual_close.
 #[global] Instance stale_qual_inst     : Stale type_qualifier := qual_fv.
 #[global] Instance subst_qual_inst     : SubstV value type_qualifier := qual_subst_one.
-#[global] Instance substM_qual_inst    : SubstM StoreT type_qualifier := qual_subst.
+#[global] Instance substM_qual_inst    : SubstM Store type_qualifier := qual_subst.
 Arguments open_qual_inst /.
 Arguments close_qual_inst /.
 Arguments stale_qual_inst /.
@@ -81,7 +81,7 @@ Notation "q1 '&q' q2" := (qualifier_and q1 q2) (at level 40).
 
 (** ** Denotation helpers *)
 
-Fixpoint eval_vals (σ : StoreT) {n} (vals : vec value n) : option (vec constant n) :=
+Fixpoint eval_vals (σ : Store) {n} (vals : vec value n) : option (vec constant n) :=
   match vals with
   | [#]       => Some [#]
   | v ::: vs  =>
@@ -95,7 +95,7 @@ Fixpoint eval_vals (σ : StoreT) {n} (vals : vec value n) : option (vec constant
       end
   end.
 
-Definition qual_interp (σ : StoreT) (q : type_qualifier) : Prop :=
+Definition qual_interp (σ : Store) (q : type_qualifier) : Prop :=
   match q with
   | qual vals prop =>
       match eval_vals σ vals with
@@ -104,10 +104,10 @@ Definition qual_interp (σ : StoreT) (q : type_qualifier) : Prop :=
       end
   end.
 
-Definition qual_interp_cl (q : type_qualifier) (σ : StoreT) : Prop :=
+Definition qual_interp_cl (q : type_qualifier) (σ : Store) : Prop :=
   qual_interp σ q.
 
-#[global] Instance denot_qual_inst : Denotation type_qualifier (StoreT → Prop) :=
+#[global] Instance denot_qual_inst : Denotation type_qualifier (Store → Prop) :=
   qual_interp_cl.
 Arguments denot_qual_inst /.
 
@@ -145,7 +145,7 @@ Lemma qual_subst_intro x v (q : type_qualifier) :
   x # q → lc_value v → {x := v}q (q ^q^ x) = {0 ~> v} q.
 Proof. Admitted.
 
-Lemma qual_interp_subst_compose (σ_X σ : StoreT) (q : type_qualifier) :
+Lemma qual_interp_subst_compose (σ_X σ : Store) (q : type_qualifier) :
   store_compat σ_X σ →
   qual_interp σ (qual_subst σ_X q) ↔ qual_interp (σ_X ∪ σ) q.
 Proof. Admitted.
