ChoiceLogic/theories/LogicQualifier.v
@@ -1,4 +1,5 @@
-From ChoicePrelude Require Import Prelude.
+From ChoiceLogic Require Import Prelude.
+From CoreLang Require Import Syntax.
 
 (** * Logic qualifiers
 
@@ -10,14 +11,14 @@ From ChoicePrelude Require Import Prelude.
     restricts both inputs to [d] before calling the predicate. *)
 
 Inductive logic_qualifier : Type :=
-  | lqual (d : aset) (prop : StoreT → WorldT → Prop).
+  | lqual (d : aset) (prop : Store → WfWorld → Prop).
 
 Definition lqual_dom (q : logic_qualifier) : aset :=
   match q with
   | lqual d _ => d
   end.
 
-Definition lqual_prop (q : logic_qualifier) : StoreT → WorldT → Prop :=
+Definition lqual_prop (q : logic_qualifier) : Store → WfWorld → Prop :=
   match q with
   | lqual _ p => p
   end.
@@ -27,8 +28,8 @@ Arguments stale_logic_qualifier /.
 
 Definition logic_qualifier_denote
     (q : logic_qualifier)
-    (σ : StoreT)
-    (w : WorldT) : Prop :=
+    (σ : Store)
+    (w : WfWorld) : Prop :=
   match q with
   | lqual d p => p (store_restrict σ d) (res_restrict w d)
   end.
